src/Verify.v
@@ -40,25 +40,32 @@ Definition newRegStateDesc : RegStateDesc :=
 Definition IntSet_to_seq_fin {n : nat} (s : IntSet) :
   all (ltn ^~ n) (IntSet_toList s) -> seq 'I_n.
 Proof.
-  elim: (IntSet_toList s) => [|x xs IHxs] /= H.
+  elim: (IntSet_toList s) => [_|? ? IHxs /andP [H ?]] /=.
     exact: [::].
-  move/andP: H => [H1 H2].
-  exact: cons (Ordinal H1) (IHxs _).
+  exact: cons (Ordinal H) (IHxs _).
 Defined.
-
-Definition RV := ('I_maxReg + 'I_maxVar)%type.
 
 Definition keepOnly {A : Type} `(xs : seq 'I_n) :
   Vec (option A) n -> Vec (option A) n :=
   vmap_with_index (fun i x => if i \in xs then x else None).
 
-Definition verifyLiveness (st : RegStateDesc) : seq 'I_maxVar -> bool :=
-  all (fun var =>
-    if vnth (rsAllocs st) var isn't Some reg  then false else
-    if vnth (rsRegs st)   reg isn't Some var' then false else
-    var == var').
+Inductive AllocError :=
+  | VarNotAllocated of VarId
+  | RegNotAllocatedToVar of nat & VarId
+  | RegAllocatedToDifferentVar of nat & VarId & VarId
+  | VarId_OutOfBounds.
 
-Definition liveRegisters (st : RegStateDesc) : seq 'I_maxVar -> seq 'I_maxReg :=
+Definition checkLiveness st : seq 'I_maxVar -> seq AllocError :=
+  flip (forFold [::]) $ fun acc var =>
+    if vnth (rsAllocs st) var isn't Some reg
+    then VarNotAllocated var :: acc
+    else if vnth (rsRegs st) reg isn't Some var'
+         then RegNotAllocatedToVar reg var :: acc
+         else if nat_of_ord var == var'
+              then acc
+              else RegAllocatedToDifferentVar reg var var' :: acc.
+
+Definition liveRegisters st : seq 'I_maxVar -> seq 'I_maxReg :=
   flip (forFold [::]) $ fun acc var =>
     if vnth (rsAllocs st) var is Some reg
     then reg :: acc
@@ -71,7 +78,7 @@ Inductive RegState : RegStateDesc -> Prop :=
      Anything other than these should not be presently active, all them should
      be active, and they should apply to the correct variables. *)
   | BlockCheck st (lives : seq 'I_maxVar) :
-    verifyLiveness st lives ->
+    size (checkLiveness st lives) == 0 ->
     RegState
       {| rsRegs   := keepOnly (liveRegisters st lives) $ rsRegs st
        ; rsAllocs := keepOnly lives $ rsAllocs st
@@ -96,38 +103,6 @@ Inductive RegState : RegStateDesc -> Prop :=
        ; rsStack  := rsStack st
        |}
 
-(*
-  | MoveReg st r1 r2 v :
-    vnth (rsRegs st) r1 == Some v ->
-    vnth (rsRegs st) r2 == None ->
-    RegState
-      {| rsRegs   := rsRegs st
-       ; rsAllocs := rsAllocs st
-       ; rsStack  := rsStack st
-       |}
-
-  | SwapReg st :
-    RegState
-      {| rsRegs   := rsRegs st
-       ; rsAllocs := rsAllocs st
-       ; rsStack  := rsStack st
-       |}
-
-  | SpillReg st :
-    RegState
-      {| rsRegs   := rsRegs st
-       ; rsAllocs := rsAllocs st
-       ; rsStack  := rsStack st
-       |}
-
-  | LoadReg st :
-    RegState
-      {| rsRegs   := rsRegs st
-       ; rsAllocs := rsAllocs st
-       ; rsStack  := rsStack st
-       |}
-*)
-
   | AllocStack st v :
     vnth (rsAllocs st) v == None ->
     vnth (rsStack  st) v == false ->
@@ -144,39 +119,99 @@ Inductive RegState : RegStateDesc -> Prop :=
       {| rsRegs   := rsRegs st
        ; rsAllocs := rsAllocs st
        ; rsStack  := vreplace (rsStack st) v false
-       |}
-
-  | UseReg st :
-    RegState
-      {| rsRegs   := rsRegs st
-       ; rsAllocs := rsAllocs st
-       ; rsStack  := rsStack st
-       |}
-
-  | SetReg st :
-    RegState
-      {| rsRegs   := rsRegs st
-       ; rsAllocs := rsAllocs st
-       ; rsStack  := rsStack st
        |}.
+
+Definition getRegStateDesc `(st : RegState rd) := rd.
+Arguments getRegStateDesc [rd] st /.
 
 Variable A : Type.
 
-Definition AllocError := nat.
+Definition VerifiedSig := { d : RegStateDesc * A | RegState (fst d) }.
+
+Definition packVerified `(st : RegState rd) (s : A) :=
+  exist (RegState \o fst) (rd, s) st.
+Arguments packVerified [rd] st s /.
 
 (* The [Verified] transformer stack uses [EitherT] to allow sudden exit due to
    error, otherwise it maintains the current [RegState] plus whatever
    additional state the user desires. *)
-Definition Verified :=
-  EitherT AllocError (StateT { d : RegStateDesc * A | RegState (fst d) } mType).
+Definition Verified := EitherT (seq AllocError) (StateT VerifiedSig mType).
 
-Definition verifyCheckBlock (liveIn : IntSet) : Verified unit := pure tt.
+Definition _rs {a b : Type} {P : a -> Prop} :
+  Getter { x : a * b | P (fst x) } a :=
+  fun _ _ _ f s => fmap (const s) (f (fst (proj1_sig s))).
+
+Definition _aside {a b : Type} {P : a -> Prop} :
+  Lens' { x : a * b | P (fst x) } b :=
+  fun _ _ f s =>
+    let: exist (x, y) H := s in
+    fmap (fun z => exist _ (x, z) H) (f y).
+
+Definition runVerified `(m : Verified b) (i : A) : mType (seq AllocError + b) :=
+  fmap fst <$> m (exist _ (newRegStateDesc, i) StartState).
+
+Definition allocReg (r : 'I_maxReg) (v : 'I_maxVar) : Verified unit := pure tt.
+
+Definition freeReg (r : 'I_maxReg) (v : 'I_maxVar) : Verified unit := pure tt.
+
+Definition allocStack (v : 'I_maxVar) : Verified unit := pure tt.
+
+Definition freeStack (v : 'I_maxVar) : Verified unit := pure tt.
+
+Definition verifyCheckBlock' (st : RegStateDesc) (s : A) (lives : IntSet) :
+  seq AllocError + VerifiedSig.
+Proof.
+  case L: (all (ltn ^~ maxVar) (IntSet_toList lives)).
+    have l := IntSet_to_seq_fin L.
+    move=> {L lives}.
+    case B: (checkLiveness st l) => [|e es].
+      have H : size (checkLiveness st l) == 0.
+        by rewrite B.
+      exact (inr (packVerified (BlockCheck H) s)).
+    exact: inl (e :: es).
+  exact: inl [:: VarId_OutOfBounds].
+Defined.
+
+Definition verifyCheckBlock (lives : IntSet) : Verified unit :=
+  pure tt.
+  (* z <-- lift $ use _ex1 ;; *)
+  (* let: (st, a) := z in *)
+  (* match verifyCheckBlock' st a lives *)
+  (* return Verified unit with *)
+  (* | inl es => pure (inl es) *)
+  (* | inr x  => lift $ putT x *)
+  (* end. *)
 
 Definition verifyApplyAllocs (op : opType1) (allocs : seq (VarId * PhysReg)) :
   Verified (seq opType2) :=
   lift $ lift $ applyAllocs oinfo op allocs.
 
 Definition verifyResolutions (moves : seq (ResolvingMove maxReg)) :
-  Verified unit := pure tt.
+  Verified unit :=
+  forM_ moves $ fun mv =>
+    match mv with
+    | Move    x y =>
+        pure tt
+    | Swap    x y =>
+        pure tt
+    | Spill   x s =>
+        pure tt
+    | Restore s x =>
+        pure tt
+    | Nop         =>
+        pure tt
+    end.
 
 End Verify.
+
+Module VerifyLensLaws.
+
+Include LensLaws.
+
+Variable a b : Type.
+Variable P : a -> Prop.
+
+(* Program Instance Lens__rs : LensLaws (@_rs a b P). *)
+Program Instance Lens__aside : LensLaws (@_aside a b P).
+
+End VerifyLensLaws.
